src/PlutusIR/Semantics/Static/normaliser/STLC_norm_completeness.v
@@ -11,8 +11,76 @@ Proof.
   (* This requires proving equivalence, likely with the definition of `strong_normalization`. *)
 Admitted. *)
 
+Lemma uhm t t' :
+  step_d_f t = t' -> True.
+Proof.
+  intros.
+  destruct (step_d_f t) eqn:Heq.
+Admitted.
+
+Lemma x :
+  normalizer'' 
+Admitted.
+
+Theorem norm_complete_mysn Δ K (t tn : term) (Hwt : SN_STLC_named.has_type Δ t K):
+  normalise t tn -> @normalizerMySN t Δ K Hwt = tn.
+Proof.
+  intros HnormR.
+  generalize dependent Δ.
+  generalize dependent K.
+  induction HnormR; intros K' Δ Hwt; subst; auto.
+  - inversion Hwt; subst.
+    specialize (IHHnormR2 K1 Δ H4).
+    specialize (IHHnormR1 (tp_arrow K1 K') Δ H2).
+    specialize (IHHnormR3 (tp_arrow K1 K') Δ).
+    admit.
+  - admit.
+  - inversion Hwt; subst.
+    specialize (IHHnormR K2 ((bX, K)::Δ) H4).
+    unfold normalizerMySN.
+    destruct (strong_normalization_mysn Hwt).
+    + unfold normalizer''.
+      unfold normalizerMySN in IHHnormR.
+      destruct (strong_normalization_mysn H4).
+      * unfold normalizer'' in IHHnormR. subst. reflexivity.
+      * (* Should yield a contradiction. 
+        If step_d_f T0 = Some t', then step_d_f (tmlam bX K T0) = Some (tmlam bX K t').
+
+
+        *)
+        inversion e.
+        unfold bind in H0.
+        assert (step_d_f T0 = None) by admit.
+        destruct s as [t' [HstepT0' HSNt'] ].
+        rewrite HstepT0' in H.
+        inversion H.      
+    + destruct s as [t' [HstepT HSNt'] ]. 
+      unfold normalizerMySN in IHHnormR.
+      destruct (strong_normalization_mysn H4) in IHHnormR.
+      * inversion HstepT.
+        unfold bind in H0.
+        assert (step_d_f T0 <> None) by admit. (* Follows from the match*)
+        contradiction.
+      * destruct s as [t'0 [HstepT0 HSNt'0] ].
+        (* unfold normalizer'' in IHHnormR. *)
+        unfold normalizer''.
+        destruct HSNt'.
+        inversion IHHnormR.
+        (* assert (t' = tmlam bX K t'0) by admit. *)
+        subst.
+        
+        f_equal.
+        subst.
+        admit.
+        admit.
+  
+  - unfold normalizerMySN.
+    destruct (strong_normalization_mysn Hwt).
+    unfold normalizer''.
+    reflexivity.
+
 Theorem norm_complete Δ K (t tn : term) (Hwt : SN_STLC_named.has_type Δ t K) :
-    normalise t tn -> normalizer Hwt = tn.
+    normalise t tn -> @normalizer t Δ K Hwt = tn.
 Proof.
     intros HnormR.
     generalize dependent Δ.
@@ -41,22 +109,33 @@ Proof.
       (* specialize (IHHnormR ((bX, K)::Δ)). *)
       inversion Hwt; subst.
       specialize (IHHnormR K2 ((bX, K)::Δ) H4).
+      unfold normalizer.
+      destruct (strong_normalization_d Hwt). 
+       (* simpl. *)
+      unfold normalizer in IHHnormR.
+      destruct (strong_normalization_d H4) in IHHnormR.
+      simpl in IHHnormR.
+       
+      (* destruct IHHnormR. *)
+      destruct (step_d_f T0) eqn:Heq.
+      
+      
+      (*
+        Suppose (step_d_f T0 = None)
+        Then normalise T0 T0 and T0n = T0.
+
+        Then also in the goal, we have that the match becomes a None, so that it becomse
+        tmlam bX K T0.
+      *)
+       
+      
+      unfold step_d_f.
+      
       admit.
     - unfold normalizer.
-      inversion Hwt; subst.
-      (* unfold normalizer''. *)
+      destruct (strong_normalization_d Hwt).
       simpl.
-      remember Hwt as Hwt'; clear HeqHwt'.
-      assert (SN (tmvar X)).
-      {
-        apply strong_normalization in Hwt'.
-        
-        apply Hwt'.
-      }
-      admit.
-      
-      
-      
+      reflexivity.  
 Admitted.
 
 Theorem norm_sound Δ T (t tn : term) (Hwt : SN_STLC_named.has_type Δ t T) :
