src/PlutusIR/Semantics/Static/normaliser/uhm.v
@@ -1,0 +1,2 @@
+From PlutusCert Require Import SN_STLC_named STLC_named.
+
